deps/poulet4/lib/P4cub/BigStep/TypeSoundness.v
@@ -35,7 +35,7 @@ Section BigStepTheorems.
 
   Section ExprPreservation.
     Local Hint Resolve eval_slice_types : core.
-    Fail Local Hint Resolve eval_uop_types : core.
+    Local Hint Resolve eval_uop_types : core.
     Local Hint Resolve eval_bop_type : core.
     Local Hint Resolve eval_cast_types : core.
     Local Hint Resolve eval_member_types : core.
