deps/poulet4/lib/P4cub/BigStep/Value/Syntax.v
@@ -25,8 +25,8 @@ Inductive v : Type :=
 | VHeaderStack (ts : F.fs string E.t)
                (headers : list (bool * F.fs string v))
                (size : positive) (nextIndex : Z)
-| VString (s : string)
-| VEnum (x m : string).
+(*| VString (s : string)
+| VEnum (x m : string)*).
 (**[]*)
 
 (** Lvalues. *)
@@ -64,10 +64,10 @@ Module ValueNotations.
   Notation "'STACK' vs : ts [ n ] 'NEXT' ':=' ni"
            := (VHeaderStack ts vs n ni)
                 (in custom p4value at level 0, no associativity).
-  Notation "'STR' s"
+  (*Notation "'STR' s"
     := (VString s) (in custom p4value at level 0).
   Notation "'ENUM' x 'DOT' m"
-    := (VEnum x m) (in custom p4value at level 0).
+    := (VEnum x m) (in custom p4value at level 0).*)
 End ValueNotations.
 
 Module LValueNotations.
