deps/poulet4/lib/P4cub/Syntax/IndPrincip.v
@@ -39,9 +39,9 @@ Section TypeInduction.
   Hypothesis HTHeaderStack : forall fields size,
       F.predfs_data P fields -> P {{ stack fields[size] }}.
 
-  Hypothesis HTString : P {{ Str }}.
+  (*Hypothesis HTString : P {{ Str }}.
 
-  Hypothesis HTEnum : forall x xs, P {{ enum x { xs } }}.
+  Hypothesis HTEnum : forall x xs, P {{ enum x { xs } }}.*)
   
   (** A custom induction principle.
       Do [induction ?t using custom_t_ind]. *)
@@ -71,8 +71,8 @@ Section TypeInduction.
       | {{ struct { fields } }} => HTStruct fields (fields_ind fields)
       | {{ hdr { fields } }} => HTHeader fields (fields_ind fields)
       | {{ stack fields[n] }} => HTHeaderStack fields n (fields_ind fields)
-      | {{ Str }} => HTString
-      | {{ enum x { xs } }} => HTEnum x xs
+      (*| {{ Str }} => HTString
+      | {{ enum x { xs } }} => HTEnum x xs*)
       end.
   (**[]*)
 End TypeInduction.
@@ -136,9 +136,9 @@ Section ExprInduction.
   Hypothesis HAccess : forall e1 e2 i,
       P e1 -> P <{ Access e1[e2] @ i }>.
 
-  Hypothesis HString : forall s i, P <{ Stri s @ i }>.
+  (*Hypothesis HString : forall s i, P <{ Stri s @ i }>.
 
-  Hypothesis HEnum : forall x m i, P <{ Enum x dot m @ i }>.
+  Hypothesis HEnum : forall x m i, P <{ Enum x dot m @ i }>.*)
   
   (** A custom induction principle.
       Do [induction ?e using custom_e_ind]. *)
@@ -177,8 +177,8 @@ Section ExprInduction.
       | <{ Stack hs:ts [n] nextIndex:=ni @ i }>
         => HEStack ts hs n ni i (list_ind hs)
       | <{ Access e1[e2] @ i }> => HAccess e1 e2 i (eind e1)
-      | <{ Stri s @ i }> => HString s i
-      | <{ Enum x dot m @ i }> => HEnum x m i
+      (*| <{ Stri s @ i }> => HString s i
+      | <{ Enum x dot m @ i }> => HEnum x m i*)
       end.
   (**[]*)
 End ExprInduction.
