deps/poulet4/lib/P4sel/P4sel.v
@@ -32,8 +32,8 @@ Module P4sel.
                (i : tags_t)                            (* error literals *)
       | EMatchKind (mk : P4cub.Expr.matchkind) (i : tags_t)       (* matchkind literals *)
       | EHeaderStackAccess (stack : e) (index : Z) (i : tags_t) (*header-stack access*)
-      | EString (s : string) (i : tags_t)
-      | EEnum (x m : string) (i : tags_t)
+      (*| EString (s : string) (i : tags_t)
+      | EEnum (x m : string) (i : tags_t)*)
       .
       (**[]*)
 
@@ -44,8 +44,8 @@ Module P4sel.
       | EExprMember _ t _ _ => t
       | EError _ _ => P4cub.Expr.TError
       | EMatchKind _ _ => P4cub.Expr.TMatchKind
-      | EString _ _ => P4cub.Expr.TString
-      | EEnum x m _ => P4cub.Expr.TEnum x [m]
+      (*| EString _ _ => P4cub.Expr.TString
+      | EEnum x m _ => P4cub.Expr.TEnum x [m]*)
       | EHeaderStackAccess stack _ _ => 
         match SelTypeOf stack with
         | P4cub.Expr.THeaderStack fields _ => 
@@ -154,9 +154,10 @@ Module P4sel.
       | SSeq (s1 s2 : s) (i : tags_t)                   (* sequences *)
       | SBlock (blk : s)                                (* blocks *)
       | SExternMethodCall (e : string) (f : string)
+                          (typ_args : list P4cub.Expr.t)
                           (args : E.arrowE tags_t)
                           (i : tags_t)                  (* extern method calls *)
-      | SFunCall (f : string)
+      | SFunCall (f : string) (typ_args : list P4cub.Expr.t)
                  (args : E.arrowE tags_t) (i : tags_t)  (* function call *)
       | SActCall (f : string)
                  (args : E.args tags_t) (i : tags_t)    (* action call *)
@@ -289,6 +290,7 @@ Module P4sel.
       (** Top-level declarations. *)
       Inductive d : Type :=
       | TPInstantiate (C : string) (x : string)
+                      (type_args : list P4cub.Expr.t)
                      (cargs : E.constructor_args tags_t)
                      (arg_init: S.s tags_t)
                      (i : tags_t) (* constructor [C] that 
@@ -297,8 +299,9 @@ Module P4sel.
                                      constructor [args]
                                      makes instance [x]. *)
       | TPExtern (e : string)
+                 (typ_params : list string)
                  (cparams : P4cub.Expr.constructor_params)
-                 (methods : F.fs string P4cub.Expr.arrowT)
+                 (methods : F.fs string (list string * P4cub.Expr.arrowT))
                  (i : tags_t) (* extern declarations *)
       | TPControl (c : string)
                   (cparams : P4cub.Expr.constructor_params) (* constructor params *)
@@ -312,9 +315,10 @@ Module P4sel.
                  (start : P.state_block tags_t) (* start state *)
                  (states : F.fs string (P.state_block tags_t)) (* parser states *)
                  (i : tags_t) (* parser declaration *)
-      | TPFunction (f : string) (signature : P4cub.Expr.arrowT) (body : S.s tags_t)
+      | TPFunction (f : string) (typ_params : list string)
+                   (signature : P4cub.Expr.arrowT) (body : S.s tags_t)
                    (i : tags_t) (* function/method declaration *)
-      | TPPackage (p : string)
+      | TPPackage (p : string) (typ_params : list string)
                   (cparams : P4cub.Expr.constructor_params) (* constructor params *)
                   (i : tags_t) (* package type declaration *)
       | TPSeq (d1 d2 : d) (i : tags_t).
